made robust-slice example work

theories/iris/examples/segment/example07import.v
@@ -15,7 +15,7 @@ Unset Printing Implicit Defensive.
 
 Close Scope byte_scope.
 
-Section Example01.
+Section Example07.
 
 
 Notation "{{{ P }}} es {{{ v , Q }}}" :=
@@ -25,45 +25,43 @@ Notation "{{{ P }}} es {{{ v , Q }}}" :=
   Context `{!wasmG Σ,
       !logrel_na_invs Σ, HHB: HandleBytes, !cinvG Σ, !cancelG Σ}.
 
-  (*
-allocate a handle h with space for one i32
-if allocation failed, set global variable g to 0 and return
-write 42 to h
-read from h
-set global variable g to the read value
-free h
-*)
-
   Definition example_program :=
     [
-      BI_const (xx 4);
-      BI_segalloc;
+      BI_get_global 1;
       BI_tee_local 0;
-      BI_isdummy;
-      BI_if (Tf [] []) [ BI_const (xx 0) ; BI_set_global 0; BI_return ] [];
-      BI_get_local 0;
       BI_const (xx 42);
       BI_segstore T_i32;
       BI_get_local 0;
       BI_segload T_i32;
-      BI_set_global 0;
-      BI_get_local 0;
-      BI_segfree
+      BI_set_global 0 
     ].
 
   Definition example_function f :=
     [ AI_local 0 f [ AI_basic (BI_block (Tf [] []) example_program) ] ].
 
 
-  Lemma program_spec f k f0 gv:
+  Lemma program_spec f k k' h f0 gv bs x:
     f.(f_inst).(inst_globs) !! 0 = Some k ->
+    f.(f_inst).(inst_globs) !! 1 = Some k' ->
     length f.(f_locs) >= 1 ->
+    valid h ->
+    (offset h + N.of_nat (t_length T_i32) <= bound h)%N ->
 
-    ⊢ {{{ ↪[frame] f0 ∗ N.of_nat k ↦[wg] {| g_mut := MUT_mut ; g_val := gv |} }}}
+    ⊢ {{{ ↪[frame] f0 ∗ N.of_nat k ↦[wg] {| g_mut := MUT_mut ; g_val := gv |}
+            ∗ N.of_nat k' ↦[wg] {| g_mut := MUT_mut ; g_val := VAL_handle h |}
+            ∗ ↦[wss][ handle_addr h ] bs ∗ ⌜ length bs = 4 ⌝
+            ∗ id h ↣[allocated] Some x
+      }}}
       example_function f
-      {{{ v, ⌜ v = immV [] ⌝ ∗ ↪[frame] f0 ∗ (∃ gv, N.of_nat k ↦[wg] {| g_mut := MUT_mut ; g_val := VAL_numeric (xx gv) |} ∗ ⌜ gv = 0 ∨ gv = 42 ⌝) }}}.
+      {{{ v, ⌜ v = immV [] ⌝
+                     ∗ ↪[frame] f0 
+                     ∗ N.of_nat k ↦[wg] {| g_mut := MUT_mut ; g_val := VAL_numeric (xx 42) |}
+                     ∗ N.of_nat k' ↦[wg] {| g_mut := MUT_mut ; g_val := VAL_handle h |}
+                     ∗ (∃ bs, ↦[wss][ handle_addr h ] bs ∗ ⌜ length bs = 4 ⌝)
+                     ∗ id h ↣[allocated] Some x
+      }}}.
   Proof.
-    iIntros (Hglob Hlocs Φ) "!> (Hf & Hg) HΦ".
+    iIntros (Hglob Hglobh Hlocs Hvalid Hoff Φ) "!> (Hf & Hg & Hgh & Hws & %Hbs & Hall) HΦ".
 
     iApply (wp_frame_bind with "Hf"); first done.
     iIntros "Hf". 
@@ -75,20 +73,14 @@ free h
     iApply wp_ctx_bind. done. 
     
     iSimpl.
-    rewrite (separate2 (AI_basic _)).
+    rewrite (separate1 (AI_basic _)).
     iApply wp_seq.
     iSplitR; last first.
-    iSplitL "Hf".
-    unfold xx. fold_const.
-    iApply (wp_wand with "[-]").
-    iApply (wp_segalloc with "[$Hf]"); first done.
-    iIntros "!>" (w) "H". iExact "H".
-    iIntros (w) "[(%h & -> & H) Hf]".
-    iSimpl.
-    instantiate (1 := λ x, ((∃ h, ⌜ x = immV [VAL_handle h] ⌝ ∗ _) ∗ ↪[frame] f)%I).
-    iSimpl. iFrame. iExists h. iSplit; first done. iExact "H".
-    2: by iIntros "[(%h & % & _) _]". 
-    iIntros (w) "[(%h & -> & Hh) Hf]".
+    iSplitL "Hf Hgh".
+    iApply (wp_get_global with "[] Hf Hgh") => //.
+    by instantiate (1 := λ x, ⌜ x = immV _ ⌝%I). 
+    2:by iIntros "[% _]". 
+    iIntros (w) "(-> & Hgh & Hf)".
 
     iSimpl. rewrite (separate2 (AI_handle h)).
     iApply wp_seq. iSplitR; last first.
@@ -104,102 +96,15 @@ free h
     2: by iIntros "[% _]".
     iIntros (w) "[-> Hf]". 
                                
-
-    iSimpl. rewrite (separate2 (AI_handle h)).
-    iApply wp_seq. iSplitR; last first.
-    iSplitL "Hf".
-    iApply (wp_isdummy with "Hf").
-    by instantiate (1 := λ x, ⌜ x = immV _ ⌝%I).
-    2: by iIntros "[% _]".
-    iIntros (w) "[-> Hf]". iSimpl.
-
-    rewrite (separate2 (AI_basic _)).
-        
-    iDestruct "Hh" as "[-> | (Ha & %Hbound & %Hoff & %Hvalid & Hs)]".
-    { (* Case 1: segalloc failed *)
-
-      iApply wp_seq.
-      iSplitR; last first.
-      iSplitL. 
-    
-      iApply (wp_if_true with "Hf"). done. 
-      iIntros "!> Hf".
-      rewrite - (app_nil_l [AI_basic _]). iApply (wp_block with "Hf") => //.
-      iIntros "!> Hf".
-      
-      iApply wp_wasm_empty_ctx. iApply wp_label_push_nil. iApply wp_ctx_bind. done.
-      iSimpl. rewrite (separate2 (AI_basic _)).
-      iApply wp_seq.
-      iSplitR; last first.
-      iSplitL "Hf Hg".
-      fold_const. iApply (wp_set_global with "[] Hf Hg"). done.
-      by instantiate (1 := λ x, ⌜ x = immV [] ⌝%I).
-      2: by iIntros "[% _]".
-      iIntros (w) "(-> & Hg & Hf)".
-      iSimpl. iApply wp_value. apply of_to_val. done.
-      iSimpl. iApply (wp_label_pull_nil _ _ _ _ _ (LH_base [] [])).
-      iApply wp_wasm_empty_ctx. 
-
-      iApply wp_value.
-      unfold IntoVal. apply language.of_to_val. done.
-      instantiate (1 := λ x, (⌜ x = retV _ ⌝ ∗ _)%I).
-      iSplit; first done.
-      iCombine "HΦ Hg Hf" as "H". iExact "H".
-      2: by iIntros "[% _]".
-      iIntros (w) "(-> & HΦ & Hg & Hf)".
-      iSimpl. iApply wp_value. apply of_to_val. done. 
-           
-      iSimpl. iApply (wp_label_pull_nil _ _ _ _ _ (LH_base [] [])).
-      iApply wp_wasm_empty_ctx. 
-      iApply wp_value. apply of_to_val. done.
-      iExists _. iFrame. iIntros "Hf". iSimpl.
-      iApply (wp_wand with "[Hf]").
-      iApply wp_return.
-      3:{ instantiate (3 := 2). instantiate (1 := []). 
-          instantiate (1 := LH_rec [] _ _ (LH_rec [] _ _ (LH_base [] []) _) []).
-          unfold lfilled, lfill. simpl. done. }
-      done. done.
-      iNext. iApply wp_value. apply of_to_val => //. iFrame.
-      by instantiate (1 := λ x, ⌜ x = immV [] ⌝%I).
-      iIntros (w) "[-> Hf]".
-      iApply "HΦ". iSplit => //. iFrame. iExists _. iFrame.
-      iPureIntro. by left. }
-
-    (* Case 2: segalloc succeeded *)
-
-    iApply wp_seq.
-    iSplitR; last first.
-    iSplitL "Hf".
-    iApply (wp_if_false with "Hf"). unfold is_dummy. rewrite Hvalid. simpl.
-    rewrite andb_false_r. simpl. done.
-    iIntros "!> Hf".
-    rewrite - (app_nil_l [AI_basic _]).
-    iApply (wp_block with "Hf") => //.
-    iIntros "!> Hf".
-    iApply (wp_label_value with "Hf"). done.
-    by instantiate (1 := λ x, ⌜ x = immV [] ⌝%I).
-    2: by iIntros "[% _]".
-    iIntros (w) "[-> Hf]". 
-
-    
-    iSimpl.
-    rewrite (separate1 (AI_basic _)).
-    iApply wp_seq. iSplitR; last first.
-    iSplitL "Hf". iApply (wp_get_local with "[] Hf").
-    simpl. rewrite set_nth_read. done.
-    by instantiate (1 := λ x, ⌜ x = immV _ ⌝ %I).
-    2: by iIntros "[% _]".
-    iIntros (w) "[-> Hf]". iSimpl.
-
+    iSimpl. 
     rewrite (separate3 (AI_handle _)). 
     
     iApply wp_seq.
     iSplitR; last first.
-    iSplitL "Hf Ha Hs".
+    iSplitL "Hf Hall Hws".
     fold_const.
-    replace (base h) with (handle_addr h); last by unfold handle_addr; rewrite Hoff; lia.
-    iApply (wp_segstore with "[$Ha $Hs $Hf]") => //.
-    rewrite Hoff Hbound. simpl. lia.
+    
+    iApply (wp_segstore with "[$Hall $Hws $Hf]") => //.
     iIntros "!> H". instantiate (1 := λ x, (⌜ x = immV [] ⌝ ∗ _)%I).
     iSplit; [done | iExact "H"].
     2: by iIntros "[[% _] _]".
@@ -216,38 +121,16 @@ free h
     iSplitL "Ha Hs Hf".
     iApply (wp_segload with "[$Ha $Hs $Hf]") => //.
     2:{ rewrite map_map. rewrite map_id. done. } 
-    done. rewrite Hoff Hbound. simpl. lia.
+    done. 
     iIntros "!> H".
     instantiate (1 := λ x, (⌜ x = immV _ ⌝ ∗ _)%I).
     iSplit; [done | iExact "H"].
     2: by iIntros "[[% _] _]".
     iIntros (w) "[(-> & Ha & Hs) Hf]". iSimpl.
-    rewrite (separate2 (AI_basic _)).
-    iApply wp_seq.
-    iSplitR; last first.
-    iSplitL "Hf Hg". 
     fold_const. 
-    iApply (wp_set_global with "[] Hf Hg").
+    iApply (wp_wand with "[Hf Hg]"). iApply (wp_set_global with "[] Hf Hg").
     done. by instantiate (1 := λ x, ⌜ x = immV [] ⌝%I).
-    2: by iIntros "[% _]". 
     iIntros (w) "(-> & Hg & Hf)".
-    iSimpl. rewrite (separate1 (AI_basic _)).
-    iApply wp_seq. iSplitR; last first.
-    iSplitL "Hf". iApply (wp_get_local with "[] Hf").
-    rewrite set_nth_read. done.
-    by instantiate (1 := λ x, ⌜ x = immV _ ⌝%I).
-    2: by iIntros "[% _]".
-    iIntros (w) "[-> Hf]".
-    iSimpl. iApply (wp_wand with "[Hf Ha Hs]").
-    unfold handle_addr. rewrite Hoff N.add_0_r.
-    rewrite - Hbound. 
-    iApply (wp_segfree with "[$Hf $Ha $Hs]") => //.
-    rewrite map_length. rewrite (length_bits _ T_i32) => //.
-    by rewrite Hbound. 
-    iIntros "!> Ha". instantiate (1 := λ x, (⌜ x = immV _ ⌝ ∗ _)%I).
-    iSplit; [done | iExact "Ha"].
-    iIntros (w) "[[-> Ha] Hf]". 
-                                                      
     
     iSimpl. iApply (wp_label_pull_nil _ _ _ _ _ (LH_base [] [])).
     iApply wp_wasm_empty_ctx.
@@ -263,13 +146,14 @@ free h
     
     iApply "HΦ". 
     iSplit; first done. iFrame. iExists _. iFrame.
-    iPureIntro. by right. 
+    iPureIntro. rewrite map_length. erewrite length_bits.
+    by instantiate (1 := T_i32). done. 
   Qed. 
     
     
-End Example01. 
+End Example07. 
 
-Section Example01Host. 
+Section Example07Host. 
   Context `{!wasmG Σ, !hvisG Σ, !hmsG Σ, !hasG Σ,
         !logrel_na_invs Σ, HHB: HandleBytes, !cancelG Σ, !cinvG Σ}.
 
@@ -309,12 +193,18 @@ Section Example01Host.
       mod_start := Some {| modstart_func := Mk_funcidx 0 |};
       mod_imports := [   {| imp_module := list_byte_of_string "Ret";
                          imp_name := list_byte_of_string "ret_glob";
-                         imp_desc := ID_global {| tg_mut := MUT_mut; tg_t := T_i32 |} |} ];
+                           imp_desc := ID_global {| tg_mut := MUT_mut; tg_t := T_i32 |} |};
+                         {| imp_module := list_byte_of_string "Han";
+                         imp_name := list_byte_of_string "handle_glob";
+                         imp_desc := ID_global {| tg_mut := MUT_mut; tg_t := T_handle |} |} ];
       mod_exports := []
     |}.
 
   Definition example_func_impts : seq.seq extern_t := [].
-  Definition example_glob_impts : seq.seq extern_t := [ET_glob {| tg_mut := MUT_mut; tg_t := T_i32 |}].
+  Definition example_glob_impts : seq.seq extern_t :=
+    [ET_glob {| tg_mut := MUT_mut; tg_t := T_i32 |};
+     ET_glob {| tg_mut := MUT_mut; tg_t := T_handle |}
+    ].
 
 
 
@@ -336,10 +226,7 @@ Section Example01Host.
     repeat split;eauto.
     { apply Forall2_cons. split;auto. cbn.
       repeat split;auto.
-      unfold example_program. rewrite (separate6 (BI_const _)).
-      eapply bet_composition'.
-      { apply/b_e_type_checker_reflects_typing => /= ; by apply/eqP. }
-      { apply/b_e_type_checker_reflects_typing => /=; by apply/eqP. } } 
+      apply/b_e_type_checker_reflects_typing => /=; by apply/eqP. }
     { apply Forall2_cons. split;auto. } 
   Qed.
 
@@ -353,56 +240,67 @@ Section Example01Host.
 
 
   Definition example_instantiate g :=
-    [ ID_instantiate [] 0 [0%N] ;
+    [ ID_instantiate [] 0 [0%N; 1%N] ;
       H_get_global g ].
 
-  Lemma instantiate_example g_ret wret (*all*):
+  Lemma instantiate_example g_ret g_han wret h:
     typeof wret = T_i32 ->
-    ⊢ {{{ ↪[frame] empty_frame ∗ (* interp_allocator all ∗ *)
+    ⊢ {{{ ↪[frame] empty_frame ∗ 
             (N.of_nat g_ret) ↦[wg] {| g_mut := MUT_mut; g_val := wret |} ∗
-             (∃ name, 0%N ↪[vis] {| modexp_name := name; modexp_desc := MED_global (Mk_globalidx g_ret) |}) ∗
+            (N.of_nat g_han) ↦[wg] {| g_mut := MUT_mut; g_val := VAL_handle h |} ∗
+            (∃ name, 0%N ↪[vis] {| modexp_name := name; modexp_desc := MED_global (Mk_globalidx g_ret) |}) ∗
+            (∃ nameh, 1%N ↪[vis] {| modexp_name := nameh; modexp_desc := MED_global (Mk_globalidx g_han) |}) ∗
             0%N ↪[mods] example_module (* ∗ 
           na_own logrel_nais ⊤ ∗ *)
       }}}
       ((example_instantiate g_ret,[]) : host_expr)
       {{{  λ v: language.val wasm_host_lang, ⌜v = immHV [xxv 0]⌝ ∨ ⌜v = immHV [xxv 42]⌝ }}} .
   Proof.
-    iIntros "%Hret !>" (Φ) "(Hf & Hg & Hexp & Hmod) HΦ".
+    iIntros "%Hret !>" (Φ) "(Hf & Hg & Hgh & Hexp & Hexph & Hmod) HΦ".
     iDestruct "Hexp" as (name) "Hexp".
-    iApply (instantiation_spec_operational_start_seq with "Hf [Hmod Hexp Hg]").
+    iDestruct "Hexph" as (nameh) "Hexph".
+    iDestruct (mapsto_ne with "Hg Hgh") as "%Hgg". 
+    
+    iApply (instantiation_spec_operational_start_seq with "Hf [Hmod Hexp Hexph Hgh Hg]").
     2: exact example_module_typing.
     2: exact module_restrictions_example.
     done. iFrame. 
-    iSplitL "Hexp". 
+    iSplitL "Hexp Hexph". 
     unfold import_resources_host => //.
-    instantiate (1 := [_]). iSimpl. iSplit; last done.
-    done.
+    instantiate (1 := [_;_]). iSimpl. iFrame. 
     iSplitL.
     iSplitL.
     iSplitR.
     repeat iSplit. 
     unfold import_func_resources => //=.
-    iPureIntro. unfold func_typecheck => //=. constructor => //. 
+    iPureIntro. unfold func_typecheck => //=. constructor => //. constructor => //. 
     iPureIntro. unfold func_domcheck => //=.
     iSplitR.
     repeat iSplit. 
     unfold import_tab_resources => //.
-    iPureIntro. unfold tab_typecheck => //=. constructor => //.
+    iPureIntro. unfold tab_typecheck => //=. constructor => //. constructor => //. 
     iPureIntro. unfold tab_domcheck => //.
     iSplitR.
     repeat iSplit. 
     unfold import_mem_resources => //.
-    iPureIntro. unfold mem_typecheck => //=. constructor => //.
+    iPureIntro. unfold mem_typecheck => //=. constructor => //. constructor => //. 
     unfold mem_domcheck => //.
-    instantiate (1 := <[ N.of_nat g_ret := _ ]> ∅).
+    instantiate (1 := <[ N.of_nat g_han := _ ]> (<[ N.of_nat g_ret := _ ]> ∅)).
     iSplitL. 
-    unfold import_glob_resources. 
+    unfold import_glob_resources.
+    iApply big_sepM_insert. by rewrite lookup_insert_ne. iFrame. 
     iApply big_sepM_singleton. iFrame. 
     unfold glob_typecheck => //. iPureIntro. split. constructor => //=.
-    eexists _,_. 
-    split; first by rewrite lookup_insert.
+    eexists _,_.
+    split. rewrite lookup_insert_ne => //. 
+    by rewrite lookup_insert.
     split; first done. 
     unfold global_agree. simpl. by rewrite Hret.
+    constructor => //=.
+    eexists _,_.
+    split; first by rewrite lookup_insert.
+    split; first done.
+    unfold global_agree. simpl. done. 
     unfold glob_domcheck => //=. by set_solver.
     iSplit; iPureIntro.
     unfold module_elem_bound_check_gmap => //. constructor => //.
@@ -423,25 +321,22 @@ Section Example01Host.
     destruct l => //.
     iDestruct "Hfuncs" as "[Hfunc _]". rewrite Hinst_types. iSimpl in "Hfunc". 
 
-    iDestruct "Himp" as "[Himp _]".
+    iDestruct "Himp" as "(Himp & Himph & _)".
     iDestruct "Hirwt" as "(Hirwtf & Hirwtm & Hirwtt & Hirwtg)".
     iDestruct "Hirwtg" as "(Hg & %Hgtypecheck & %Hgdomcheck)".
     unfold import_glob_resources.
+    iDestruct (big_sepM_insert with "Hg") as "[Hgh Hg]".
+    by rewrite lookup_insert_ne. 
     iDestruct big_sepM_singleton as "[Hsing _]". 
     iDestruct ("Hsing" with "Hg") as "Hg".
     iClear "Hsing". 
-    
+
     simpl in Hglobinit.
-(*    assert (exists v, glob_allocs = [ {| g_mut := MUT_mut; g_val := VAL_numeric v |} ])
-      as [gv ->].
-    { destruct g_inits; eexists => //. }
-    
-    iDestruct (big_sepL2_length with "Hglobs") as "%Hlenglobs".
-    unfold get_import_global_count in Hlenglobs. simpl in Hlenglobs.
-    rewrite drop_0 in Hlenglobs. *)
     destruct (inst_globs inst) eqn:Hglobs => //.
     { inversion Hextglob. simpl in H. done. }
-    inversion Hextglob. simpl in H. inversion H; subst g. 
+    destruct l.
+    { inversion Hextglob. simpl in H. done. } 
+    inversion Hextglob. simpl in H. inversion H; subst g g0. 
 
     (* iDestruct "Hglobs" as "[Hg _]".  *)
 
@@ -453,18 +348,20 @@ Section Example01Host.
     rewrite - (app_nil_l [AI_invoke _]).
     iApply (wp_invoke_native with "Hf Hfunc") => //.
     iIntros "!> [Hf Hfunc]".
-    iApply (program_spec with "[$Hf $Hg]") => //=.
-    by rewrite Hglobs. lia.
-    iIntros (w) "(-> & Hf & H)". iDestruct "H" as (gf) "[Hg %Hgf]".
+    iApply (program_spec with "[$Hf Hg Hgh]") => //=.
+    by rewrite Hglobs. by rewrite Hglobs. lia.
+    admit. admit. iFrame. admit. 
+(*    iExists _. done. *)
+    iIntros (w) "(-> & Hf & H)". iDestruct "H" as "(Hg & Hghan & Hss & Hall)".
     iSimpl.
     iApply (wp_get_global_host _ _ _ _ [] with "Hg").
     iIntros "!> Hg".
     iApply "HΦ". iSimpl.
-    destruct Hgf as [-> | ->]; [by iLeft | by iRight].
-  Qed. 
+    by iRight. 
+  Admitted. 
 
     
     
     
     
-End Example01Host.
+End Example07Host.
