theories/iris/examples/segment/example10slicefree.v
@@ -15,7 +15,7 @@ Unset Printing Implicit Defensive.
 
 Close Scope byte_scope.
 
-Section Example01.
+Section Example10.
 
 
 Notation "{{{ P }}} es {{{ v , Q }}}" :=
@@ -25,29 +25,34 @@ Notation "{{{ P }}} es {{{ v , Q }}}" :=
   Context `{!wasmG Σ,
       !logrel_na_invs Σ, HHB: HandleBytes, !cinvG Σ, !cancelG Σ}.
 
-  (*
-allocate a handle h with space for one i32
-if allocation failed, set global variable g to 0 and return
-write 42 to h
-read from h
-set global variable g to the read value
-free h
+
+(* 
+allocate a handle (h 0) with space for two i32s
+if allocation failed, trap
+slice it into halves (h' 1) and (h'' 2)
+free (h'' 2)
 *)
 
+
+  
   Definition example_program :=
     [
-      BI_const (xx 4);
+      BI_const (xx 8);
       BI_segalloc;
       BI_tee_local 0;
       BI_isdummy;
-      BI_if (Tf [] []) [ BI_const (xx 0) ; BI_set_global 0; BI_return ] [];
+      BI_if (Tf [] []) [ BI_unreachable ] [];
       BI_get_local 0;
-      BI_const (xx 42);
-      BI_segstore T_i32;
+      BI_const (xx 0);
+      BI_const (xx 4);
+      BI_slice;
+      BI_set_local 1;
       BI_get_local 0;
-      BI_segload T_i32;
-      BI_set_global 0;
-      BI_get_local 0;
+      BI_const (xx 4);
+      BI_const (xx 4);
+      BI_slice;
+      BI_set_local 2;
+      BI_get_local 2;
       BI_segfree
     ].
 
@@ -55,15 +60,14 @@ free h
     [ AI_local 0 f [ AI_basic (BI_block (Tf [] []) example_program) ] ].
 
 
-  Lemma program_spec f k f0 gv:
-    f.(f_inst).(inst_globs) !! 0 = Some k ->
-    length f.(f_locs) >= 1 ->
+  Lemma program_spec f f0:
+    length f.(f_locs) >= 3 ->
 
-    ⊢ {{{ ↪[frame] f0 ∗ N.of_nat k ↦[wg] {| g_mut := MUT_mut ; g_val := gv |} }}}
+    ⊢ {{{ ↪[frame] f0 }}}
       example_function f
-      {{{ v, ⌜ v = immV [] ⌝ ∗ ↪[frame] f0 ∗ (∃ gv, N.of_nat k ↦[wg] {| g_mut := MUT_mut ; g_val := VAL_numeric (xx gv) |} ∗ ⌜ gv = 0 ∨ gv = 42 ⌝) }}}.
+      {{{ v, ⌜ v = trapV ⌝ }}}.
   Proof.
-    iIntros (Hglob Hlocs Φ) "!> (Hf & Hg) HΦ".
+    iIntros (Hlocs Φ) "!> Hf HΦ".
 
     iApply (wp_frame_bind with "Hf"); first done.
     iIntros "Hf". 
@@ -95,7 +99,7 @@ free h
     iSplitL "Hf". fold_const. iApply (wp_tee_local with "Hf").
     iIntros "!> Hf". rewrite (separate1 (AI_const _)).
     iApply (wp_val_app). done. iSplitR; last first.
-    iApply (wp_wand with "[Hf]"). iApply (wp_set_local with "[] Hf"). done.
+    iApply (wp_wand with "[Hf]"). iApply (wp_set_local with "[] Hf"). lia. 
     by instantiate (1 := λ x, ⌜ x = immV [] ⌝%I).
     iIntros (w) "[-> Hf]". iSimpl.
     instantiate (1 := λ x, (⌜ x = immV _ ⌝ ∗ _)%I).
@@ -118,52 +122,35 @@ free h
     iDestruct "Hh" as "[-> | (Ha & %Hbound & %Hoff & %Hvalid & Hs)]".
     { (* Case 1: segalloc failed *)
 
-      iApply wp_seq.
-      iSplitR; last first.
-      iSplitL. 
-    
+      iApply (wp_wand with "[Hf]"). iApply wp_seq_trap.
+      iFrame. iIntros "Hf". 
+      
       iApply (wp_if_true with "Hf"). done. 
       iIntros "!> Hf".
       rewrite - (app_nil_l [AI_basic _]). iApply (wp_block with "Hf") => //.
       iIntros "!> Hf".
       
       iApply wp_wasm_empty_ctx. iApply wp_label_push_nil. iApply wp_ctx_bind. done.
-      iSimpl. rewrite (separate2 (AI_basic _)).
-      iApply wp_seq.
-      iSplitR; last first.
-      iSplitL "Hf Hg".
-      fold_const. iApply (wp_set_global with "[] Hf Hg"). done.
-      by instantiate (1 := λ x, ⌜ x = immV [] ⌝%I).
-      2: by iIntros "[% _]".
-      iIntros (w) "(-> & Hg & Hf)".
-      iSimpl. iApply wp_value. apply of_to_val. done.
+      iSimpl.
+      iApply (wp_wand with "[Hf]"). iApply (wp_unreachable with "Hf").
+      by instantiate (1 := λ x, ⌜ x = trapV ⌝%I). 
+      iIntros (w) "(-> & Hf)".
       iSimpl. iApply (wp_label_pull_nil _ _ _ _ _ (LH_base [] [])).
-      iApply wp_wasm_empty_ctx. 
+      iApply wp_wasm_empty_ctx.
 
-      iApply wp_value.
-      unfold IntoVal. apply language.of_to_val. done.
-      instantiate (1 := λ x, (⌜ x = retV _ ⌝ ∗ _)%I).
-      iSplit; first done.
-      iCombine "HΦ Hg Hf" as "H". iExact "H".
-      2: by iIntros "[% _]".
-      iIntros (w) "(-> & HΦ & Hg & Hf)".
-      iSimpl. iApply wp_value. apply of_to_val. done. 
-           
+      iApply (wp_label_trap with "Hf"). done.
+      done. 
+      iIntros (w)  "(-> & Hf)".
       iSimpl. iApply (wp_label_pull_nil _ _ _ _ _ (LH_base [] [])).
-      iApply wp_wasm_empty_ctx. 
-      iApply wp_value. apply of_to_val. done.
-      iExists _. iFrame. iIntros "Hf". iSimpl.
-      iApply (wp_wand with "[Hf]").
-      iApply wp_return.
-      3:{ instantiate (3 := 2). instantiate (1 := []). 
-          instantiate (1 := LH_rec [] _ _ (LH_rec [] _ _ (LH_base [] []) _) []).
-          unfold lfilled, lfill. simpl. done. }
-      done. done.
-      iNext. iApply wp_value. apply of_to_val => //. iFrame.
-      by instantiate (1 := λ x, ⌜ x = immV [] ⌝%I).
+      iApply wp_wasm_empty_ctx.
+      iApply (wp_wand with "[Hf]"). iApply (wp_label_trap with "Hf").
+      done. by instantiate (1 := λ x, ⌜ x = trapV ⌝%I).
       iIntros (w) "[-> Hf]".
-      iApply "HΦ". iSplit => //. iFrame. iExists _. iFrame.
-      iPureIntro. by left. }
+      iExists _. iFrame. iIntros "Hf". iSimpl.
+      iApply (wp_wand with "[Hf]"). iApply (wp_frame_trap with "Hf").
+      by instantiate (1 := λ x, ⌜ x = trapV ⌝%I).
+      iIntros (w) "[-> Hf]". iApply "HΦ". done. 
+    }
 
     (* Case 2: segalloc succeeded *)
 
@@ -182,94 +169,90 @@ free h
     iIntros (w) "[-> Hf]". 
 
     
-    iSimpl.
-    rewrite (separate1 (AI_basic _)).
-    iApply wp_seq. iSplitR; last first.
-    iSplitL "Hf". iApply (wp_get_local with "[] Hf").
-    simpl. rewrite set_nth_read. done.
-    by instantiate (1 := λ x, ⌜ x = immV _ ⌝ %I).
-    2: by iIntros "[% _]".
-    iIntros (w) "[-> Hf]". iSimpl.
-
-    rewrite (separate3 (AI_handle _)). 
-    
-    iApply wp_seq.
-    iSplitR; last first.
-    iSplitL "Hf Ha Hs".
-    fold_const.
-    replace (base h) with (handle_addr h); last by unfold handle_addr; rewrite Hoff; lia.
-    iApply (wp_segstore with "[$Ha $Hs $Hf]") => //.
-    rewrite Hoff Hbound. simpl. lia.
-    iIntros "!> H". instantiate (1 := λ x, (⌜ x = immV [] ⌝ ∗ _)%I).
-    iSplit; [done | iExact "H"].
-    2: by iIntros "[[% _] _]".
-    iIntros (w) "[(-> & Ha & Hs) Hf]". iSimpl. 
-    rewrite (separate1 (AI_basic _)).
-    iApply wp_seq. iSplitR; last first.
-    iSplitL "Hf". iApply (wp_get_local with "[] Hf").
-    simpl. rewrite set_nth_read. done.
-    by instantiate (1 := λ x, ⌜ x = immV _ ⌝ %I).
-    2: by iIntros "[% _]".
-    iIntros (w) "[-> Hf]". iSimpl.
-    rewrite (separate2 (AI_handle _)).
-    iApply wp_seq. iSplitR; last first.
-    iSplitL "Ha Hs Hf".
-    iApply (wp_segload with "[$Ha $Hs $Hf]") => //.
-    2:{ rewrite map_map. rewrite map_id. done. } 
-    done. rewrite Hoff Hbound. simpl. lia.
-    iIntros "!> H".
-    instantiate (1 := λ x, (⌜ x = immV _ ⌝ ∗ _)%I).
-    iSplit; [done | iExact "H"].
-    2: by iIntros "[[% _] _]".
-    iIntros (w) "[(-> & Ha & Hs) Hf]". iSimpl.
-    rewrite (separate2 (AI_basic _)).
-    iApply wp_seq.
-    iSplitR; last first.
-    iSplitL "Hf Hg". 
-    fold_const. 
-    iApply (wp_set_global with "[] Hf Hg").
-    done. by instantiate (1 := λ x, ⌜ x = immV [] ⌝%I).
-    2: by iIntros "[% _]". 
-    iIntros (w) "(-> & Hg & Hf)".
     iSimpl. rewrite (separate1 (AI_basic _)).
     iApply wp_seq. iSplitR; last first.
     iSplitL "Hf". iApply (wp_get_local with "[] Hf").
-    rewrite set_nth_read. done.
+    simpl. rewrite set_nth_read. done.
+    by instantiate (1 := λ x, ⌜ x = immV _ ⌝%I).
+    2: by iIntros "[% _]". 
+    iIntros (w) "[-> Hf]". iSimpl.
+    rewrite (separate4 (AI_handle _)).
+    iApply wp_seq. iSplitR; last first.
+    iSplitL "Hf". 
+         
+    iApply (wp_slice with "Hf") => //=.
+    unfold slice_handle. rewrite Hbound. simpl. done. 
     by instantiate (1 := λ x, ⌜ x = immV _ ⌝%I).
     2: by iIntros "[% _]".
+    iIntros (w) "[-> Hf]". iSimpl.
+
+    rewrite (separate2 (AI_handle _)).
+    iApply wp_seq.
+    iSplitR; last first.
+    iSplitL "Hf". fold_const. iApply (wp_set_local with "[] Hf").
+    simpl. destruct (f_locs f); try by simpl in Hlocs; lia.
+    repeat (destruct l; first by simpl in Hlocs; lia). simpl. lia.
+    by instantiate (1 := λ x, ⌜ x = immV [] ⌝%I). iSimpl.
+    2: by iIntros "[% _]". 
     iIntros (w) "[-> Hf]".
-    iSimpl. iApply (wp_wand with "[Hf Ha Hs]").
-    unfold handle_addr. rewrite Hoff N.add_0_r.
-    rewrite - Hbound. 
-    iApply (wp_segfree with "[$Hf $Ha $Hs]") => //.
-    rewrite map_length. rewrite (length_bits _ T_i32) => //.
-    by rewrite Hbound. 
-    iIntros "!> Ha". instantiate (1 := λ x, (⌜ x = immV _ ⌝ ∗ _)%I).
-    iSplit; [done | iExact "Ha"].
-    iIntros (w) "[[-> Ha] Hf]". 
-                                                      
-    
-    iSimpl. iApply (wp_label_pull_nil _ _ _ _ _ (LH_base [] [])).
-    iApply wp_wasm_empty_ctx.
-    iApply (wp_wand with "[Hf]").
-    iApply (wp_label_value with "Hf"). done.
-    by instantiate (1 := λ x, ⌜ x = immV [] ⌝%I).
-    iIntros (w) "[-> Hf]".
-    iExists _. iFrame. iIntros "Hf".
-    iSimpl. iApply (wp_wand with "[Hf]").
-    iApply (wp_frame_value with "Hf"). done. done.
-    by instantiate (1 := λ x, ⌜ x = immV [] ⌝%I).
+
+     iSimpl. rewrite (separate1 (AI_basic _)).
+    iApply wp_seq. iSplitR; last first.
+    iSplitL "Hf". iApply (wp_get_local with "[] Hf").
+    simpl. remember (f_locs f) as l.
+    repeat (destruct l; first by simpl in Hlocs; lia). simpl. done. 
+    by instantiate (1 := λ x, ⌜ x = immV _ ⌝%I).
+    2: by iIntros "[% _]". 
+    iIntros (w) "[-> Hf]". iSimpl.
+    rewrite (separate4 (AI_handle _)).
+    iApply wp_seq. iSplitR; last first.
+    iSplitL "Hf". 
+         
+    iApply (wp_slice with "Hf") => //=.
+    unfold slice_handle. rewrite Hbound. simpl. done. 
+    by instantiate (1 := λ x, ⌜ x = immV _ ⌝%I).
+    2: by iIntros "[% _]".
+    iIntros (w) "[-> Hf]". iSimpl.
+
+    rewrite (separate2 (AI_handle _)).
+    iApply wp_seq.
+    iSplitR; last first.
+    iSplitL "Hf". fold_const. iApply (wp_set_local with "[] Hf").
+    simpl. destruct (f_locs f); try by simpl in Hlocs; lia.
+    repeat (destruct l; first by simpl in Hlocs; lia). simpl. lia.
+    by instantiate (1 := λ x, ⌜ x = immV [] ⌝%I). iSimpl.
+    2: by iIntros "[% _]". 
     iIntros (w) "[-> Hf]". 
     
-    iApply "HΦ". 
-    iSplit; first done. iFrame. iExists _. iFrame.
-    iPureIntro. by right. 
+
+
+    iSimpl. rewrite (separate1 (AI_basic _)).
+    iApply wp_seq. iSplitR; last first.
+    iSplitL "Hf". iApply (wp_get_local with "[] Hf").
+    simpl. remember (f_locs f) as l. repeat (destruct l; first by simpl in Hlocs; lia). done. 
+    by instantiate (1 := λ x, ⌜ x = immV _ ⌝ %I).
+    2: by iIntros "[% _]".
+    iIntros (w) "[-> Hf]". iSimpl.
+    iApply (wp_wand with "[Hf Ha]"). iApply (wp_segfree_failure2 with "[$Hf Ha]").
+    2:{ iSimpl. iFrame. iIntros "!> Ha". instantiate (1 := λ x, (⌜ x = trapV ⌝ ∗ _)%I).
+        iSplit; [done | iExact "Ha"]. }
+    simpl. lia.
+    iIntros (w) "[[-> Ha] Hf]".
+     iSimpl. iApply (wp_label_pull_nil _ _ _ _ _ (LH_base [] [])).
+     iApply wp_wasm_empty_ctx.
+     iApply (wp_wand with "[Hf]"). iApply (wp_label_trap with "Hf").
+     done. by instantiate (1 := λ x, ⌜ x = trapV ⌝%I).
+     iIntros (w) "[-> Hf]".
+     iExists _. iFrame. iIntros "Hf". iSimpl.
+     iApply (wp_wand with "[Hf]"). iApply (wp_frame_trap with "Hf").
+     by instantiate (1 := λ x, ⌜ x = trapV ⌝%I).
+     iIntros (w) "[-> Hf]". iApply "HΦ". done. 
   Qed. 
     
     
-End Example01. 
+End Example10. 
 
-Section Example01Host. 
+Section Example10Host. 
   Context `{!wasmG Σ, !hvisG Σ, !hmsG Σ, !hasG Σ,
         !logrel_na_invs Σ, HHB: HandleBytes, !cancelG Σ, !cinvG Σ}.
 
@@ -298,7 +281,7 @@ Section Example01Host.
     {| mod_types := [Tf [] []];
        mod_funcs :=  [ {|
           modfunc_type := Mk_typeidx 0 ;
-          modfunc_locals := [T_handle] ;
+          modfunc_locals := [T_handle; T_handle; T_handle] ;
           modfunc_body := example_program
         |} ] ;
       mod_tables := [];
@@ -307,14 +290,12 @@ Section Example01Host.
       mod_elem := [];
       mod_data := [];
       mod_start := Some {| modstart_func := Mk_funcidx 0 |};
-      mod_imports := [   {| imp_module := list_byte_of_string "Ret";
-                         imp_name := list_byte_of_string "ret_glob";
-                         imp_desc := ID_global {| tg_mut := MUT_mut; tg_t := T_i32 |} |} ];
+      mod_imports := [];
       mod_exports := []
     |}.
 
   Definition example_func_impts : seq.seq extern_t := [].
-  Definition example_glob_impts : seq.seq extern_t := [ET_glob {| tg_mut := MUT_mut; tg_t := T_i32 |}].
+  Definition example_glob_impts : seq.seq extern_t := []. 
 
 
 
@@ -340,7 +321,7 @@ Section Example01Host.
       eapply bet_composition'.
       { apply/b_e_type_checker_reflects_typing => /= ; by apply/eqP. }
       { apply/b_e_type_checker_reflects_typing => /=; by apply/eqP. } } 
-    { apply Forall2_cons. split;auto. } 
+    { constructor. } 
   Qed.
 
    Lemma module_restrictions_example:
@@ -352,62 +333,27 @@ Section Example01Host.
   Qed.
 
 
-  Definition example_instantiate g :=
-    [ ID_instantiate [] 0 [0%N] ;
-      H_get_global g ].
+  Definition example_instantiate :=
+    [ ID_instantiate [] 0 [] ]. 
 
-  Lemma instantiate_example g_ret wret (*all*):
-    typeof wret = T_i32 ->
-    ⊢ {{{ ↪[frame] empty_frame ∗ (* interp_allocator all ∗ *)
-            (N.of_nat g_ret) ↦[wg] {| g_mut := MUT_mut; g_val := wret |} ∗
-             (∃ name, 0%N ↪[vis] {| modexp_name := name; modexp_desc := MED_global (Mk_globalidx g_ret) |}) ∗
-            0%N ↪[mods] example_module (* ∗ 
-          na_own logrel_nais ⊤ ∗ *)
+
+  Lemma instantiate_example :
+    ⊢ {{{ ↪[frame] empty_frame ∗ 
+            0%N ↪[mods] example_module 
       }}}
-      ((example_instantiate g_ret,[]) : host_expr)
-      {{{  λ v: language.val wasm_host_lang, ⌜v = immHV [xxv 0]⌝ ∨ ⌜v = immHV [xxv 42]⌝ }}} .
+      ((example_instantiate,[]) : host_expr)
+      {{{  λ v: language.val wasm_host_lang, ⌜v = trapHV ⌝ }}}. 
   Proof.
-    iIntros "%Hret !>" (Φ) "(Hf & Hg & Hexp & Hmod) HΦ".
-    iDestruct "Hexp" as (name) "Hexp".
-    iApply (instantiation_spec_operational_start_seq with "Hf [Hmod Hexp Hg]").
+    iIntros "!>" (Φ) "(Hf & Hmod) HΦ".
+    iApply (instantiation_spec_operational_start_seq with "Hf [$Hmod]").
     2: exact example_module_typing.
     2: exact module_restrictions_example.
-    done. iFrame. 
-    iSplitL "Hexp". 
+    done. repeat iSplit ; try by iPureIntro; try constructor.  
     unfold import_resources_host => //.
-    instantiate (1 := [_]). iSimpl. iSplit; last done.
-    done.
-    iSplitL.
-    iSplitL.
-    iSplitR.
-    repeat iSplit. 
     unfold import_func_resources => //=.
-    iPureIntro. unfold func_typecheck => //=. constructor => //. 
-    iPureIntro. unfold func_domcheck => //=.
-    iSplitR.
-    repeat iSplit. 
     unfold import_tab_resources => //.
-    iPureIntro. unfold tab_typecheck => //=. constructor => //.
-    iPureIntro. unfold tab_domcheck => //.
-    iSplitR.
-    repeat iSplit. 
     unfold import_mem_resources => //.
-    iPureIntro. unfold mem_typecheck => //=. constructor => //.
-    unfold mem_domcheck => //.
-    instantiate (1 := <[ N.of_nat g_ret := _ ]> ∅).
-    iSplitL. 
-    unfold import_glob_resources. 
-    iApply big_sepM_singleton. iFrame. 
-    unfold glob_typecheck => //. iPureIntro. split. constructor => //=.
-    eexists _,_. 
-    split; first by rewrite lookup_insert.
-    split; first done. 
-    unfold global_agree. simpl. by rewrite Hret.
-    unfold glob_domcheck => //=. by set_solver.
-    iSplit; iPureIntro.
-    unfold module_elem_bound_check_gmap => //. constructor => //.
-    unfold module_data_bound_check_gmap => //. constructor => //.
-    iSplit => //. 
+    unfold import_glob_resources => //. 
     unfold export_ownership_host => //. 
     iIntros (id) "Hf (Hmod & Himp & %inst & Hpost & Hexp)".
     iDestruct "Hpost" as (??????) "(Hirwt & %Htypr & %Htabinits & %Hwts'0 & %Hbounds_elem & %Hmem_init & %Hwms0' & %Hbounds_data & %Hglobsr & %Hglobinit & Hfuncs & Htabs & Hmems & Hglobs)".
@@ -423,28 +369,6 @@ Section Example01Host.
     destruct l => //.
     iDestruct "Hfuncs" as "[Hfunc _]". rewrite Hinst_types. iSimpl in "Hfunc". 
 
-    iDestruct "Himp" as "[Himp _]".
-    iDestruct "Hirwt" as "(Hirwtf & Hirwtm & Hirwtt & Hirwtg)".
-    iDestruct "Hirwtg" as "(Hg & %Hgtypecheck & %Hgdomcheck)".
-    unfold import_glob_resources.
-    iDestruct big_sepM_singleton as "[Hsing _]". 
-    iDestruct ("Hsing" with "Hg") as "Hg".
-    iClear "Hsing". 
-    
-    simpl in Hglobinit.
-(*    assert (exists v, glob_allocs = [ {| g_mut := MUT_mut; g_val := VAL_numeric v |} ])
-      as [gv ->].
-    { destruct g_inits; eexists => //. }
-    
-    iDestruct (big_sepL2_length with "Hglobs") as "%Hlenglobs".
-    unfold get_import_global_count in Hlenglobs. simpl in Hlenglobs.
-    rewrite drop_0 in Hlenglobs. *)
-    destruct (inst_globs inst) eqn:Hglobs => //.
-    { inversion Hextglob. simpl in H. done. }
-    inversion Hextglob. simpl in H. inversion H; subst g. 
-
-    (* iDestruct "Hglobs" as "[Hg _]".  *)
-
 
     unfold check_start in Hstart. simpl in Hstart. rewrite Hfuncs in Hstart.
     move/eqP in Hstart. inversion Hstart; subst f. 
@@ -453,18 +377,14 @@ Section Example01Host.
     rewrite - (app_nil_l [AI_invoke _]).
     iApply (wp_invoke_native with "Hf Hfunc") => //.
     iIntros "!> [Hf Hfunc]".
-    iApply (program_spec with "[$Hf $Hg]") => //=.
-    by rewrite Hglobs. lia.
-    iIntros (w) "(-> & Hf & H)". iDestruct "H" as (gf) "[Hg %Hgf]".
-    iSimpl.
-    iApply (wp_get_global_host _ _ _ _ [] with "Hg").
-    iIntros "!> Hg".
-    iApply "HΦ". iSimpl.
-    destruct Hgf as [-> | ->]; [by iLeft | by iRight].
+    iApply (program_spec with "[$Hf]") => //=.
+    lia.
+    iIntros (w) "->". iApply iris_host.wp_value. done.
+    iApply "HΦ". done. 
   Qed. 
 
     
     
     
     
-End Example01Host.
+End Example10Host.
