theories/interpreter.v
@@ -485,7 +485,7 @@ Definition run_one_step (call : run_stepE ~> itree (run_stepE +' eff))
           expect
             (find_and_remove h.(id) s.(s_alls).(allocated))
             (fun '(l, a, n) =>
-               if ((a == h.(base)))%N then
+               if ((a == h.(base)) && (n == h.(bound)))%N then
                  ret (upd_s_all s {| allocated := l; next_free := next_free s.(s_alls) |}, f, RS_normal (vs_to_es ves'))
                else ret (s, f, crash_error))
             (ret (s, f, crash_error))
