theories/iris/examples/segment/example11pointerarithfree.v
@@ -1,0 +1,308 @@
+From mathcomp Require Import ssreflect eqtype seq ssrbool.
+From iris.program_logic Require Import language.
+From iris.proofmode Require Import base tactics classes.
+From iris.base_logic Require Export gen_heap ghost_map proph_map.
+From iris.base_logic.lib Require Export fancy_updates.
+Require Export iris iris_locations iris_properties iris_atomicity stdpp_aux.
+Require Export iris_host iris_rules iris_fundamental iris_wp iris_interp_instance_alloc.
+Require Export iris_example_helper proofmode.
+Require Export datatypes operations properties opsem.
+Require Export type_checker_reflects_typing.
+
+Set Implicit Arguments.
+Unset Strict Implicit.
+Unset Printing Implicit Defensive.
+
+Close Scope byte_scope.
+
+Section Example11.
+
+
+Notation "{{{ P }}} es {{{ v , Q }}}" :=
+  (□ ∀ Φ, P -∗ (∀ v, Q -∗ Φ v) -∗ WP (es : iris.expr) @ NotStuck ; ⊤ {{ v, Φ v }})%I (at level 50).
+
+
+  Context `{!wasmG Σ,
+      !logrel_na_invs Σ, HHB: HandleBytes, !cinvG Σ, !cancelG Σ}.
+
+
+(* 
+allocate a handle (h 0) with space for two i32s
+define (h' 1) as h+4
+free (h' 1)
+*)
+
+
+  
+  Definition example_program :=
+    [
+      BI_const (xx 8);
+      BI_segalloc;
+      BI_set_local 0;
+(*      BI_isdummy;
+      BI_if (Tf [] []) [ BI_unreachable ] []; 
+      BI_get_local 0; *)
+      BI_const (xx 4);
+      BI_get_local 0;
+      BI_handleadd;
+      BI_tee_local 1;
+      BI_segfree
+    ].
+
+  Definition example_function f :=
+    [ AI_local 0 f [ AI_basic (BI_block (Tf [] []) example_program) ] ].
+
+
+  Lemma program_spec f f0:
+    length f.(f_locs) >= 2 ->
+
+    ⊢ {{{ ↪[frame] f0 }}}
+      example_function f
+      {{{ v, ⌜ v = trapV ⌝ }}}.
+  Proof.
+    iIntros (Hlocs Φ) "!> Hf HΦ".
+
+    iApply (wp_frame_bind with "Hf"); first done.
+    iIntros "Hf". 
+    rewrite - (app_nil_l [AI_basic _]).
+    iApply (wp_block with "Hf") => //.
+    iIntros "!> Hf".
+    iApply wp_wasm_empty_ctx.
+    iApply wp_label_push_nil.
+    iApply wp_ctx_bind. done. 
+    
+    iSimpl.
+    rewrite (separate2 (AI_basic _)).
+    iApply wp_seq.
+    iSplitR; last first.
+    iSplitL "Hf".
+    unfold xx. fold_const.
+    iApply (wp_wand with "[-]").
+    iApply (wp_segalloc with "[$Hf]"); first done.
+    iIntros "!>" (w) "H". iExact "H".
+    iIntros (w) "[(%h & -> & H) Hf]".
+    iSimpl.
+    instantiate (1 := λ x, ((∃ h, ⌜ x = immV [VAL_handle h] ⌝ ∗ _) ∗ ↪[frame] f)%I).
+    iSimpl. iFrame. iExists h. iSplit; first done. iExact "H".
+    2: by iIntros "[(%h & % & _) _]". 
+    iIntros (w) "[(%h & -> & Hh) Hf]".
+
+    iSimpl. rewrite (separate2 (AI_handle h)).
+    iApply wp_seq. iSplitR; last first.
+    iSplitL "Hf". fold_const. iApply (wp_set_local with "[] Hf").
+    lia. 
+    by instantiate (1 := λ x, ⌜ x = immV [] ⌝%I).
+    2: by iIntros "[% _]". 
+    iIntros (w) "[-> Hf]". iSimpl.
+    
+                               
+
+    iSimpl. rewrite (separate2 (AI_basic _)).
+    iApply wp_seq. iSplitR; last first.
+    iSplitL "Hf".
+    rewrite (separate1 (AI_basic _)).
+    iApply wp_val_app. done.
+    iSplitR; last first.
+    iApply (wp_wand with "[Hf]"). iApply (wp_get_local with "[] Hf").
+    rewrite set_nth_read. done.
+    by instantiate (1 := λ x, ⌜ x = immV _ ⌝%I).
+    iIntros (w) "[-> Hf]".
+    instantiate (1 := λ x, (⌜ x = immV _ ⌝ ∗ _)%I).
+    iSplit; [done | iExact "Hf"].
+    by iIntros "!> [% _]". 
+    2: by iIntros "[% _]".
+    iIntros (w) "[-> Hf]". iSimpl.
+
+    rewrite (separate3 (AI_basic _)).
+    iApply wp_seq. iSplitR; last first.
+    iSplitL "Hf". iApply (wp_handleadd with "Hf").
+    unfold handle_add. simpl. assert (Z.of_N (offset h) >= 0)%Z; first lia.
+    rewrite Wasm_int.Int32.signed_repr. 
+    assert (0 <= Z.of_N (offset h) + 4)%Z; first lia.
+    apply Z.leb_le in H0. rewrite - Z.geb_leb in H0.
+    rewrite H0. done.
+    done. by instantiate (1 := λ x, ⌜ x = immV _ ⌝%I).
+    2: by iIntros "[% _]". 
+    iIntros (w) "[-> Hf]". iSimpl.
+    rewrite (separate2 (AI_handle _)).
+    iApply wp_seq. iSplitR; last first.
+    iSplitL "Hf". fold_const. iApply (wp_tee_local with "Hf").
+    iIntros "!> Hf". rewrite (separate1 (AI_const _)).
+    iApply (wp_val_app). done. iSplitR; last first.
+    iApply (wp_wand with "[Hf]"). iApply (wp_set_local with "[] Hf").
+    remember (f_locs f) as l. repeat (destruct l; first by simpl in Hlocs; lia).
+    done. 
+    by instantiate (1 := λ x, ⌜ x = immV [] ⌝%I).
+    iIntros (w) "[-> Hf]". iSimpl.
+    instantiate (1 := λ x, (⌜ x = immV _ ⌝ ∗ _)%I).
+    iSplit; first done. iExact "Hf".
+    by iIntros "!> [% _]".
+    2: by iIntros "[% _]".
+    iIntros (w) "[-> Hf]". 
+    iSimpl.
+    iDestruct "Hh" as "[-> | (Ha & %Hbound & %Hoff & %Hvalid & Hs)]".
+    { (* case 1: the allocation failed *)
+      iApply (wp_wand with "[Hf]"). iApply (wp_segfree_failure1 with "[$Hf]").
+      by right. by instantiate (1 := λ x, ⌜ x = trapV ⌝%I).
+      iIntros (w) "[-> Hf]". iApply (wp_label_pull_nil _ _ _ _ _ (LH_base [] [])).
+      iApply wp_wasm_empty_ctx. iApply (wp_wand with "[Hf]").
+      iApply (wp_label_trap with "Hf"). done. by instantiate (1 := λ x, ⌜ x = trapV ⌝%I).
+      iIntros (w) "[-> Hf]". iExists _. iFrame. iIntros "Hf".
+      iApply (wp_wand with "[Hf]"). iApply (wp_frame_trap with "Hf").
+      by instantiate (1 := λ x, ⌜ x = trapV ⌝%I).
+      iIntros (w) "[-> Hf]". iApply "HΦ". done. } 
+    (* case 2: the allocation succeeded *)
+    iApply (wp_wand with "[Hf]"). iApply (wp_segfree_failure1 with "[$Hf]").
+    left. simpl. rewrite Hoff. lias.
+    by instantiate (1 := λ x, ⌜ x = trapV ⌝%I).
+    iIntros (w) "[-> Hf]".
+    iSimpl. iApply (wp_label_pull_nil _ _ _ _ _ (LH_base [] [])).
+    iApply wp_wasm_empty_ctx.
+    iApply (wp_wand with "[Hf]"). iApply (wp_label_trap with "Hf").
+    done. by instantiate (1 := λ x, ⌜ x = trapV ⌝%I).
+    iIntros (w) "[-> Hf]".
+    iExists _. iFrame. iIntros "Hf". iSimpl.
+    iApply (wp_wand with "[Hf]"). iApply (wp_frame_trap with "Hf").
+    by instantiate (1 := λ x, ⌜ x = trapV ⌝%I).
+    iIntros (w) "[-> Hf]". iApply "HΦ". done. 
+  Qed. 
+  
+    
+End Example11. 
+
+Section Example11Host. 
+  Context `{!wasmG Σ, !hvisG Σ, !hmsG Σ, !hasG Σ,
+        !logrel_na_invs Σ, HHB: HandleBytes, !cancelG Σ, !cinvG Σ}.
+
+  Notation "{{{ P }}} es {{{ v , Q }}}" :=
+    (□ ∀ Φ, P -∗ (∀ v, Q -∗ Φ v) -∗ WP (es : host_expr) @ NotStuck ; ⊤ {{ v, Φ v }})%I (at level 50).
+  Notation "{{{ P }}} es {{{ Q }}}" :=
+    (□ ∀ Φ, P -∗ (∀ v, Q v -∗ Φ v) -∗ WP (es : host_expr) @ NotStuck ; ⊤ {{ v, Φ v }})%I (at level 50).
+
+
+  Notation " n ↪[vis]{ q } v" := (ghost_map_elem (V := module_export) visGName n q v%V)
+                           (at level 20, q at level 5, format " n ↪[vis]{ q } v") .
+  Notation " n ↪[vis] v" := (ghost_map_elem (V := module_export) visGName n (DfracOwn 1) v%V)
+                          (at level 20, format " n ↪[vis] v").
+  
+  Notation " n ↪[mods]{ q } v" := (ghost_map_elem (V := module) msGName n q v%V)
+                           (at level 20, q at level 5, format " n ↪[mods]{ q } v") .
+  Notation " n ↪[mods] v" := (ghost_map_elem (V := module) msGName n (DfracOwn 1) v%V)
+                               (at level 20, format " n ↪[mods] v").
+
+  Lemma wp_wand_host s E (e : host_expr) (Φ Ψ : language.val wasm_host_lang -> iProp Σ) :
+    WP e @ s; E {{ Φ }} -∗ (∀ v, Φ v -∗ Ψ v) -∗ WP e @ s; E {{ Ψ }}.
+  Proof. iApply (weakestpre.wp_wand). Qed.
+
+
+    Definition example_module :=
+    {| mod_types := [Tf [] []];
+       mod_funcs :=  [ {|
+          modfunc_type := Mk_typeidx 0 ;
+          modfunc_locals := [T_handle; T_handle; T_handle] ;
+          modfunc_body := example_program
+        |} ] ;
+      mod_tables := [];
+      mod_mems := [];
+      mod_globals := [];
+      mod_elem := [];
+      mod_data := [];
+      mod_start := Some {| modstart_func := Mk_funcidx 0 |};
+      mod_imports := [];
+      mod_exports := []
+    |}.
+
+  Definition example_func_impts : seq.seq extern_t := [].
+  Definition example_glob_impts : seq.seq extern_t := []. 
+
+
+
+
+  Ltac type_next :=
+  match goal with
+  | |- context [ be_typing _ ?e _  ] =>
+      rewrite -(list.take_drop (length e - 1) e);simpl take; simpl drop;
+      eapply bet_composition;[|econstructor;eauto];simpl
+  end.
+
+
+  
+  Lemma example_module_typing :
+    module_typing example_module (example_func_impts ++ example_glob_impts)
+      []. 
+  Proof. 
+    exists [Tf [] []],[ (* {| tg_mut := MUT_mut; tg_t := T_i32 |} *) ]. simpl.
+    repeat split;eauto.
+    { apply Forall2_cons. split;auto. cbn.
+      repeat split;auto.
+      unfold example_program. rewrite (separate6 (BI_const _)).
+      eapply bet_composition'.
+      { apply/b_e_type_checker_reflects_typing => /= ; by apply/eqP. }
+      { apply/b_e_type_checker_reflects_typing => /=; by apply/eqP. } } 
+    { constructor. } 
+  Qed.
+
+   Lemma module_restrictions_example:
+    module_restrictions example_module.
+  Proof.
+    unfold module_restrictions.
+    repeat split; try by exists [] => //=.
+(*                           exists [xx 99]. done.  *)
+  Qed.
+
+
+  Definition example_instantiate :=
+    [ ID_instantiate [] 0 [] ]. 
+
+
+  Lemma instantiate_example :
+    ⊢ {{{ ↪[frame] empty_frame ∗ 
+            0%N ↪[mods] example_module 
+      }}}
+      ((example_instantiate,[]) : host_expr)
+      {{{  λ v: language.val wasm_host_lang, ⌜v = trapHV ⌝ }}}. 
+  Proof.
+    iIntros "!>" (Φ) "(Hf & Hmod) HΦ".
+    iApply (instantiation_spec_operational_start_seq with "Hf [$Hmod]").
+    2: exact example_module_typing.
+    2: exact module_restrictions_example.
+    done. repeat iSplit ; try by iPureIntro; try constructor.  
+    unfold import_resources_host => //.
+    unfold import_func_resources => //=.
+    unfold import_tab_resources => //.
+    unfold import_mem_resources => //.
+    unfold import_glob_resources => //. 
+    unfold export_ownership_host => //. 
+    iIntros (id) "Hf (Hmod & Himp & %inst & Hpost & Hexp)".
+    iDestruct "Hpost" as (??????) "(Hirwt & %Htypr & %Htabinits & %Hwts'0 & %Hbounds_elem & %Hmem_init & %Hwms0' & %Hbounds_data & %Hglobsr & %Hglobinit & Hfuncs & Htabs & Hmems & Hglobs)".
+
+    simpl in Htypr.
+    destruct Htypr as (Hinst_types & Hextfunc & Hexttab & Hextmem & Hextglob & Hstart).
+
+    
+    iDestruct (big_sepL2_length with "Hfuncs") as "%Hlenfuncs".
+    unfold get_import_func_count in Hlenfuncs. simpl in Hlenfuncs.
+    rewrite drop_0 in Hlenfuncs.
+    destruct (inst_funcs inst) eqn:Hfuncs => //.
+    destruct l => //.
+    iDestruct "Hfuncs" as "[Hfunc _]". rewrite Hinst_types. iSimpl in "Hfunc". 
+
+
+    unfold check_start in Hstart. simpl in Hstart. rewrite Hfuncs in Hstart.
+    move/eqP in Hstart. inversion Hstart; subst f. 
+
+    iApply wp_lift_wasm.
+    rewrite - (app_nil_l [AI_invoke _]).
+    iApply (wp_invoke_native with "Hf Hfunc") => //.
+    iIntros "!> [Hf Hfunc]".
+    iApply (program_spec with "[$Hf]") => //=.
+    lia.
+    iIntros (w) "->". iApply iris_host.wp_value. done.
+    iApply "HΦ". done. 
+  Qed. 
+
+    
+    
+    
+    
+End Example11Host.
