theories/iris/rules/iris_rules_pure.v
@@ -35,6 +35,7 @@ Proof.
 Qed. *)
 
 
+
 (* numerics *)
 Lemma wp_unop (s : stuckness) (E : coPset) (Φ : iris.val -> iProp Σ) (v v' : value) (t: value_type) (op: unop) f0:
   app_unop op v = v' ->
